Move some generic code to a separate file

src/Dafny/jrnl/jrnl.s.dfy
@@ -1,5 +1,7 @@
 include "../machine/machine.s.dfy"
 include "../util/pow.dfy"
+include "../util/collections.dfy"
+include "kinds.s.dfy"
 
 /*
 Spec for sequential journal API, assuming we're using 2PL.
@@ -9,78 +11,9 @@ type Blkno = nat
 datatype Addr = Addr(blkno: Blkno, off: nat)
 type Object = seq<byte>
 
-// NOTE: we would like kinds to be represented by their size in bits directly,
-// but expressing that a kind is a power of two would be complicated, so we
-// define them as the power of two. This is easier to work with but annoying to
-// construct.
-type Kind = k:int | 0 <= k <= 15
-
-const KindByte: Kind := 3
-const KindUInt64: Kind := KindByte + 3
-const KindInode: Kind := KindByte + 7 // 2^7 = 128 bytes
-
 function method objSize(obj: Object): nat
 {
     |obj| * 8
-}
-
-function method kindSize(k: Kind): (sz:nat)
-ensures sz > 0
-{
-    pow_nonneg(2, k);
-    pow_pos(2, k);
-    pow(2,k)
-}
-
-function kindCount(k: Kind): nat
-{
-    pow_nonneg(2, 15-k);
-    pow(2, 15-k)
-}
-
-lemma kindSize_and_kindCount_sensible(k: Kind)
-ensures kindSize(k) * kindCount(k) == 4096*8
-{
-    assert 4096*8 == pow(2, 15);
-    pow_plus(2, k, 15-k);
-}
-
-lemma kindSize_bounds(k: Kind)
-ensures kindSize(k) <= 4096*8
-{
-    pow_increasing(2, k, 15);
-    assert pow(2,15) == 4096*8;
-}
-
-lemma lemma_kind_at_least_byte_iff(k: Kind)
-ensures kindSize(k)/8*8 == kindSize(k) <==> k >= 3
-{
-    if k >= 3 {
-        pow_plus(2, k-3, 3);
-    } else {
-        if k == 0 {
-        } else if k == 1 {
-        } else if k == 2 {
-        }
-    }
-}
-
-lemma lemma_kind_at_least_byte(k: Kind)
-requires k >= 3
-ensures kindSize(k)/8*8 == kindSize(k)
-{
-    lemma_kind_at_least_byte_iff(k);
-}
-
-function method
-repeat<T>(x: T, count: nat): (xs:seq<T>) decreases count
-ensures |xs| == count && forall i :: 0 <= i < |xs| ==> xs[i] == x
-{
-    if count == 0 then [] else [x] + repeat(x, count-1)
-}
-
-function method map_domain<K, V>(m: map<K, V>): set<K> {
-    set k:K | k in m
 }
 
 function method zeroObject(k: Kind): (obj:Object)
