src/Dafny/util/marshal.i.dfy
@@ -1,5 +1,6 @@
 include "../machine/machine.s.dfy"
 include "../machine/int_encoding.s.dfy"
+include "../util/collections.dfy"
 
 datatype Encodable = EncUInt64(x:uint64)
 
@@ -30,35 +31,6 @@ ensures seq_encode(es1 + es2) == seq_encode(es1) + seq_encode(es2)
         // NOTE(tej): discovered with a calc statement
         assert ([es1[0]] + es1[1..] + es2)[1..] == es1[1..] + es2;
     }
-}
-
-predicate prefix_of<T>(s1: seq<T>, s2: seq<T>) {
-    |s1| <= |s2| && s1 == s2[..|s1|]
-}
-
-lemma prefix_of_concat2<T>(s1: seq<T>, s2: seq<T>, s: seq<T>)
-requires prefix_of(s1, s2)
-ensures prefix_of(s1, s2 + s)
-{
-}
-
-lemma prefix_of_refl<T>(s: seq<T>)
-ensures prefix_of(s, s)
-{
-}
-
-lemma prefix_of_refl_inv<T>(s1: seq<T>, s2: seq<T>)
-requires prefix_of(s1, s2)
-requires |s1| == |s2|
-ensures s1 == s2
-{
-}
-
-lemma prefix_of_app2<T>(s1: seq<T>, s2: seq<T>, n: nat)
-requires prefix_of(s1, s2)
-requires n <= |s1|
-ensures prefix_of(s1[n..], s2[n..])
-{
 }
 
 class {:autocontracts} Encoder
