src/Dafny/jrnl/kinds.s.dfy
@@ -1,0 +1,59 @@
+include "../util/pow.dfy"
+
+// NOTE: we would like kinds to be represented by their size in bits directly,
+// but expressing that a kind is a power of two would be complicated, so we
+// define them as the power of two. This is easier to work with but annoying to
+// construct.
+type Kind = k:int | 0 <= k <= 15
+
+const KindByte: Kind := 3
+const KindUInt64: Kind := KindByte + 3
+const KindInode: Kind := KindByte + 7 // 2^7 = 128 bytes
+
+function method kindSize(k: Kind): (sz:nat)
+ensures sz > 0
+{
+    pow_nonneg(2, k);
+    pow_pos(2, k);
+    pow(2,k)
+}
+
+function kindCount(k: Kind): nat
+{
+    pow_nonneg(2, 15-k);
+    pow(2, 15-k)
+}
+
+lemma kindSize_and_kindCount_sensible(k: Kind)
+ensures kindSize(k) * kindCount(k) == 4096*8
+{
+    assert 4096*8 == pow(2, 15);
+    pow_plus(2, k, 15-k);
+}
+
+lemma kindSize_bounds(k: Kind)
+ensures kindSize(k) <= 4096*8
+{
+    pow_increasing(2, k, 15);
+    assert pow(2,15) == 4096*8;
+}
+
+lemma lemma_kind_at_least_byte_iff(k: Kind)
+ensures kindSize(k)/8*8 == kindSize(k) <==> k >= 3
+{
+    if k >= 3 {
+        pow_plus(2, k-3, 3);
+    } else {
+        if k == 0 {
+        } else if k == 1 {
+        } else if k == 2 {
+        }
+    }
+}
+
+lemma lemma_kind_at_least_byte(k: Kind)
+requires k >= 3
+ensures kindSize(k)/8*8 == kindSize(k)
+{
+    lemma_kind_at_least_byte_iff(k);
+}
