src/Dafny/util/collections.dfy
@@ -1,0 +1,45 @@
+// repeat
+
+function method
+repeat<T>(x: T, count: nat): (xs:seq<T>) decreases count
+ensures |xs| == count && forall i :: 0 <= i < |xs| ==> xs[i] == x
+{
+    if count == 0 then [] else [x] + repeat(x, count-1)
+}
+
+// map to domain as a set
+
+function method map_domain<K, V>(m: map<K, V>): set<K> {
+    set k:K | k in m
+}
+
+// prefix_of
+
+predicate prefix_of<T>(s1: seq<T>, s2: seq<T>) {
+    |s1| <= |s2| && s1 == s2[..|s1|]
+}
+
+lemma prefix_of_concat2<T>(s1: seq<T>, s2: seq<T>, s: seq<T>)
+requires prefix_of(s1, s2)
+ensures prefix_of(s1, s2 + s)
+{
+}
+
+lemma prefix_of_refl<T>(s: seq<T>)
+ensures prefix_of(s, s)
+{
+}
+
+lemma prefix_of_refl_inv<T>(s1: seq<T>, s2: seq<T>)
+requires prefix_of(s1, s2)
+requires |s1| == |s2|
+ensures s1 == s2
+{
+}
+
+lemma prefix_of_app2<T>(s1: seq<T>, s2: seq<T>, n: nat)
+requires prefix_of(s1, s2)
+requires n <= |s1|
+ensures prefix_of(s1[n..], s2[n..])
+{
+}
